connect deterministic validator, parser and serializer to the API

src/cbor/pulse/CBOR.Pulse.API.Det.fsti
@@ -26,6 +26,77 @@ val cbor_det_match_with_size_eq:
       pure (sz == Seq.length (Spec.cbor_det_serialize v))
     )
 
+noextract [@@noextract_to "krml"]
+let cbor_det_validate_post
+  (v: Seq.seq U8.t)
+  (res: SZ.t)
+: Tot prop
+=
+      if SZ.v res = 0
+      then (~ (exists v1 v2 . v == Spec.cbor_det_serialize v1 `Seq.append` v2))
+      else (exists v1 v2 . v == Spec.cbor_det_serialize v1 `Seq.append` v2 /\ SZ.v res == Seq.length (Spec.cbor_det_serialize v1))
+
+val cbor_det_validate
+  (input: S.slice U8.t)
+  (#pm: perm)
+  (#v: Ghost.erased (Seq.seq U8.t))
+: stt SZ.t
+    (pts_to input #pm v)
+    (fun res -> pts_to input #pm v ** pure (
+      cbor_det_validate_post v res
+    ))
+
+val cbor_det_parse
+  (input: S.slice U8.t)
+  (len: SZ.t)
+  (#pm: perm)
+  (#v: Ghost.erased (Seq.seq U8.t))
+: stt cbor_det_t
+    (pts_to input #pm v ** pure (
+      exists v1 v2 . Ghost.reveal v == Spec.cbor_det_serialize v1 `Seq.append` v2 /\ SZ.v len == Seq.length (Spec.cbor_det_serialize v1)
+    ))
+    (fun res -> exists* v' .
+      cbor_det_match 1.0R res v' **
+      Trade.trade (cbor_det_match 1.0R res v') (pts_to input #pm v) ** pure (
+        SZ.v len <= Seq.length v /\
+        Seq.slice v 0 (SZ.v len) == Spec.cbor_det_serialize v'
+    ))
+
+noextract [@@noextract_to "krml"]
+let cbor_det_size_post
+  (bound: SZ.t)
+  (y: Spec.cbor)
+  (res: SZ.t)
+: Tot prop
+=
+      let s = Seq.length (Spec.cbor_det_serialize y) in
+      (SZ.v res == 0 <==> s > SZ.v bound) /\
+      (SZ.v res > 0 ==> SZ.v res == s)
+
+val cbor_det_size
+  (x: cbor_det_t)
+  (bound: SZ.t)
+  (#y: Ghost.erased Spec.cbor)
+  (#pm: perm)
+: stt SZ.t
+    (cbor_det_match pm x y)
+    (fun res -> cbor_det_match pm x y ** pure (
+      cbor_det_size_post bound y res
+    ))
+
+val cbor_det_serialize
+  (x: cbor_det_t)
+  (output: S.slice U8.t)
+  (#y: Ghost.erased Spec.cbor)
+  (#pm: perm)
+: stt SZ.t
+    (exists* v . cbor_det_match pm x y ** pts_to output v ** pure (Seq.length (Spec.cbor_det_serialize y) <= SZ.v (S.len output)))
+    (fun res -> exists* v . cbor_det_match pm x y ** pts_to output v ** pure (
+      let s = Spec.cbor_det_serialize y in
+      SZ.v res == Seq.length s /\
+      (exists v' . v `Seq.equal` (s `Seq.append` v'))
+    ))
+
 val cbor_det_map_entry_match: perm -> cbor_det_map_entry_t -> Spec.cbor & Spec.cbor -> slprop
 
 val cbor_det_mk_map () : mk_map_t cbor_det_match cbor_det_map_entry_match
